Comparse.Bytes.fsti
@@ -3,6 +3,9 @@ module Comparse.Bytes
 open FStar.Mul
 open FStar.UInt //Bring in scope the `pow2_values` lemma
 
+val find_nbytes: n:nat -> Pure pos (requires True)
+  (ensures fun res -> (n == 0 /\ res == 1) \/ (pow2 (8 * (res-1)) <= n /\ n < pow2 (8 * res)))
+
 type nat_lbytes (sz:nat) = n:nat{n < pow2 (8*sz)}
 
 /// Minimal interface to manipulate symbolic bytes.
